finished proof that eutt respects eqit_secure

theories/Secure/SecureEq.v
@@ -49,6 +49,7 @@ Section SecureUntimed.
   Context (priv : forall A, E A -> L).
   Context (RR : R1 -> R2 -> Prop).
 
+
   Inductive secure_eqitF (b1 b2 : bool) (l : L) vclo (sim : itree E R1 -> itree E R2 -> Prop) : itree' E R1 -> itree' E R2 -> Prop := 
 
     (* eqitF constructors *)
@@ -69,10 +70,14 @@ Section SecureUntimed.
     | EqVisUnPrivLInd {A} (e : E A) k1 t2 (CHECK : b1) (SECCHECK : ~ leq (priv A e) l) :
         (forall a, secure_eqitF b1 b2 l vclo sim (observe (k1 a)) (observe t2) ) ->
         secure_eqitF b1 b2 l vclo sim (VisF e k1) (observe t2)
-    | EqVisUnPrivRLInd {A} (e : E A) t1 k2 (CHECK : b2) (SECCHECK : ~ leq (priv A e) l) :
+    | EqVisUnPrivRInd {A} (e : E A) t1 k2 (CHECK : b2) (SECCHECK : ~ leq (priv A e) l) :
         (forall a, secure_eqitF b1 b2 l vclo sim (observe t1) (observe (k2 a) )) ->
         secure_eqitF b1 b2 l vclo sim (observe t1) (VisF e k2)
     (*| (halt : E A) k (Hempty : empty A) (r) : forall r', RR r' r -> eqit_secure (Vis halt k) (Ret r)
+      SecureOutput
+
+      cofix t := Vis SecretOutput (fun _ => t)
+      cofix t := Tau t ≅ Tau Tau Tau ...
 
      *)
   .
@@ -120,6 +125,10 @@ Section SecureUntimed.
 
 End SecureUntimed.
 
+Hint Resolve secure_eqit_mono : paco.
+
+Hint Constructors secure_eqitF : core.
+
 Definition NatPreorder : Preorder :=
   {|
   L := nat;
@@ -135,6 +144,23 @@ Section SecureUntimedUnReflexive.
 
 . 
 
+(* 
+CoInductive itree E R :=
+...
+| Vis {A : Type} (e : E A) (k : A -> itree E R)
+
+suppose A := void
+
+k ≅ empty_cont
+
+bind (Vis Halt k1) k2 ≅ Vis Halt k1 
+
+E := HaltE unit
+
+Definition halt : itree E R := Vis HaltE (fun _ => Tau Tau ...)
+
+*)
+
   Definition priv_counter : forall A, NonDet A -> nat :=
     fun _ e =>
       match e with
@@ -147,7 +173,7 @@ Section SecureUntimedUnReflexive.
   Variant Exc : Type -> Type :=
     Throw : Exc void.
 
-  Definition refl_counter : itree NonDet bool := trigger SecureFlip.
+  Definition refl_counter : itree NonDet bool := trigger SecureFlip. (* b := Flip; return b *)
 
   Lemma refl_counter_counter : ~ eqit_secure NatPreorder priv_counter eq true true 0 refl_counter refl_counter.
     Proof.
@@ -172,10 +198,592 @@ Section SecureUntimedUnReflexive.
     Qed.
     (*transitivity problems in presence of E void *)
     Definition refl_counter2 : itree NonDet unit := ITree.bind refl_counter (fun b : bool => if b then Ret tt else trigger PublicOut).
-
+    (* b := SecretFlip; if b then return tt else PublicOut; return tt*)
     Lemma refl_counter2_counter : ~ eqit_secure NatPreorder priv_counter eq true true 0 refl_counter2 refl_counter2.
       Proof.
-        Admitted.
+        unfold refl_counter2. intro Hcontra. punfold Hcontra; try eapply secure_eqit_mono; eauto.
+        red in Hcontra. cbn in Hcontra. inv Hcontra; ITrace.inj_existT; subst.
+        - inv SECCHECK.
+        - specialize (H0 true false). pclearbot. punfold H0; try eapply secure_eqit_mono; eauto.
+          red in H0. cbn in *. inv H0; ITrace.inj_existT; subst.
+          cbn in *. apply SECCHECK; auto.
+        - rewrite H3 in H0; clear H3. specialize (H0 true). cbn in *.
+          inv H0; ITrace.inj_existT; subst; ITrace.inj_existT.
+          specialize (H2 false). rewrite H in H2. cbn in *. inv H2; 
+          ITrace.inj_existT; subst; apply SECCHECK1; constructor.
+        - rewrite <- H0 in H. injection H; intros; ITrace.inj_existT; subst; ITrace.inj_existT; subst.
+          specialize (H1 true). inv H1; ITrace.inj_existT; subst.
+          rewrite H6 in H3. specialize (H3 false). cbn in *.
+          inv H3; ITrace.inj_existT; subst. apply SECCHECK1; constructor.
+      Qed.
+          
+
+Section eqit_secureC.
+  (* might not be the order I eventually want but whatever*)
+  Context {E: Type -> Type} {R1 R2 : Type} (RR : R1 -> R2 -> Prop).
+  Context (Label : Preorder) (priv : forall A, E A -> L) (l : L).
+
+
+  Variant eqit_secure_trans_clo (b1 b2 b1' b2' : bool) (r : itree E R1 -> itree E R2 -> Prop) : 
+    itree E R1 -> itree E R2 -> Prop :=
+        eqit_secure_trans_clo_intro t1 t2 t1' t2' RR1 RR2
+      (EQVl: eqit_secure Label priv RR1 b1 b1' l t1 t1')
+      (EQVr: eqit_secure Label priv RR2 b2 b2' l t2 t2')
+      (REL: r t1' t2')
+      (LERR1: forall x x' y, RR1 x x' -> RR x' y -> RR x y)
+      (LERR2: forall x y y', RR2 y y' -> RR x y' -> RR x y) :
+      eqit_secure_trans_clo b1 b2 b1' b2' r t1 t2.
+
+  Hint Constructors eqit_secure_trans_clo : core.
+
+  Definition eqit_secureC b1 b2 := eqit_secure_trans_clo b1 b2 false false.
+  Hint Unfold eqit_secureC : core.
+
+  Lemma eqit_secureC_mon b1 b2 r1 r2 t1 t2 
+    (IN : eqit_secureC b1 b2 r1 t1 t2)
+    (LE: r1 <2= r2) : 
+    eqit_secureC b1 b2 r2 t1 t2.
+  Proof.
+    destruct IN; eauto.
+  Qed.
+
+
+  
+
+End eqit_secureC.
+(*
+Lemma eqit_secureC_wcompat :  forall b1 b2 E R1 R2 (RR : R1 -> R2 -> Prop ) vclo
+      Label priv l
+      (MON : monotone2 vclo)
+      (CMP : compose (eqit_secureC RR Label priv l b1 b2) vclo <3= 
+             compose vclo (eqit_secureC RR Label priv l b1 b2))
+, (forall A, E A -> nonempty A) -> wcompatible2 (@secure_eqit_ E R1 R2 Label priv RR b1 b2 l vclo) 
+                                         (eqit_secureC RR Label priv l b1 b2) .
+Proof.
+  (*Pay attention to where you use the nonempty condition, this might be false*)
+  intros. constructor.
+  { red. intros; eapply eqit_secureC_mon; eauto. }
+  intros. dependent induction PR. 
+  (* figure out the monotone thing*)
+  punfold EQVl. punfold EQVr. red in EQVl. red in EQVr.
+  red in REL. red. hinduction REL before r; intros; clear t1' t2'.
+  - remember (RetF r1) as x. hinduction EQVl before r; intros; subst; try inv Heqx; eauto.
+    remember (RetF r3) as y. hinduction EQVr before r; intros; subst; try inv Heqy; eauto.
+    (* EqVisUnPrivRLInd slight problem with syntactic form of the constructor,
+       nothing deep *)
+    remember (RetF r1) as rr1. assert (rr1 = observe (Ret r1)); subst; auto.
+    rewrite H4. constructor; eauto. intros. eapply H1; eauto.
+  - unfold compose in CMP. remember (TauF t1) as x. hinduction EQVl before r; intros; subst; try inv Heqx;
+    try inv CHECK; eauto.
+    + remember (TauF t4) as y. pclearbot. 
+      (* think I might have a lead on the problem, should H0 have vclo not id here?*)
+      hinduction EQVr before r; intros; subst; try inv Heqy;
+      try inv CHECK; pclearbot; eauto.
+      * constructor. gclo. econstructor; eauto with paco.
+      * eapply EqVisUnPrivTauRCo; eauto. intros. 
+        eapply MON;
+           try (intros; eapply gpaco2_clo; auto; apply PR).
+        eapply CMP.
+        econstructor; try eapply H0; eauto.
+        (* in analogous case in other proof, I had more evidence about vclo
+           seems like it should be coming from a coinductive case somewhere around here
+         *)
+        (* this seems problematic, perhaps I use vclo in some incorrect way
+           if vclo was specialized to id, this would be fine*)
+        admit.
+      * assert (TauF t1 = observe (Tau t1)); auto. rewrite H4. eapply EqVisUnPrivRLInd; eauto.
+        intros. eapply H1; eauto.
+    + pclearbot. remember (TauF t3) as y.
+      hinduction EQVr before r; intros; inv Heqy; try inv CHECK; subst; eauto.
+      * pclearbot. apply EqVisUnPrivTauLCo; auto. intros. eapply MON.
+        -- eapply CMP. econstructor; try apply H1; eauto.
+           (* r vclo issue *) admit.
+        -- intros. gclo.
+      admit. (*Iwant b1 to be true here but O don't know if it is *)
+      * admit.
+      * admit.
+  - inv CHECK. remember (TauF t1) as x. 
+    hinduction EQVl before r; intros; try inv Heqx; try inv CHECK; subst; eauto. 
+    + constructor; eauto. eapply IHREL; eauto. pclearbot. punfold H0.
+    + constructor; eauto; intros. eapply IHREL; eauto. specialize (H0 a).
+      pclearbot. punfold H0.
+  - inv CHECK. remember (TauF t2) as y.
+    hinduction EQVr before r; intros; try inv Heqy; try inv CHECK; subst; eauto.
+    + constructor; auto. eapply IHREL; eauto. pclearbot. punfold H0.
+    + constructor; auto. intros. specialize (H0 a). pclearbot. punfold H0.
+  - remember (VisF e k1) as x.
+    hinduction EQVl before r; intros; try inv Heqx; try inv CHECK; subst; 
+    ITrace.inj_existT; subst; eauto.
+    + pclearbot. remember (VisF e0 k3) as y.
+      hinduction EQVr before r; intros; try inv Heqy; try inv CHECK; subst;
+      ITrace.inj_existT; subst; eauto.
+      * constructor; auto. intros. eapply MON.
+        -- eapply CMP. pclearbot. econstructor; eauto; try apply H0. apply H1.
+        -- intros. apply gpaco2_clo; auto.
+      * pclearbot. assert (TauF t1 = observe (Tau t1) ); auto. rewrite H3. 
+        eapply EqVisUnPrivTauLCo; eauto. intros.
+        eapply MON.
+        -- eapply CMP. pclearbot. econstructor; eauto.
+           apply H1. apply H0.
+        -- intros. apply gpaco2_clo; auto.
+      * pclearbot. eapply EqVisUnPrivVisCo; eauto. intros.
+        eapply MON.
+        -- eapply CMP. pclearbot. red. econstructor; eauto.
+           apply H1. apply H0.
+        -- intros. apply gpaco2_clo; auto.
+      * (* inductive case *) 
+        assert (VisF e0 k0 = observe (Vis e0 k0)); auto. rewrite H4.
+        remember (Vis e0 k0) as t. constructor; auto; subst. intros.
+        eapply H1; eauto. 
+    + pclearbot. remember (VisF e0 k0) as x.
+      hinduction EQVr before r; intros; subst; try inv Heqx; try inv CHECK;
+      ITrace.inj_existT; subst; try contradiction; eauto.
+    + pclearbot. remember (VisF e k3) as x.
+      hinduction EQVr before r; intros; subst; try inv Heqx; try inv CHECK;
+      ITrace.inj_existT; subst; try contradiction; eauto.
+  - remember (VisF e k1) as x. 
+    hinduction EQVl before r; intros; subst; try inv Heqx; try inv CHECK; ITrace.inj_existT; subst; 
+    try contradiction.
+    + constructor; eauto.
+    + pclearbot. remember (TauF t2) as y.
+      hinduction EQVr before r; intros; subst; try inv Heqy; try inv CHECK;
+      ITrace.inj_existT; subst; eauto.
+      * constructor. apply gpaco2_clo. pclearbot.
+        assert (nonempty A0); auto. inv H3.
+        econstructor; eauto. apply H1.
+        Unshelve. all : auto.
+        (* seems like I can just go through and do all of these manually, annoying but doable*)
+        (* basically reverse of the other problem need to prove r but have vclo r*)
+        admit.
+      *  eapply EqVisUnPrivTauRCo; eauto. intros.
+         eapply MON.
+         -- eapply CMP; eauto. econstructor; eauto.
+            apply H1. pclearbot. apply H0.
+         -- intros. apply gpaco2_clo. auto.
+      * assert (TauF t0 = observe (Tau t0)); auto. rewrite H4.
+        eapply EqVisUnPrivRLInd; eauto. intros. eapply H1; eauto.
+   + pclearbot. remember (TauF t2) as y.
+      hinduction EQVr before r; intros; subst; try inv Heqy; try inv CHECK;
+      ITrace.inj_existT; subst; eauto.
+      * pclearbot. apply EqVisUnPrivTauLCo; auto.
+        intros. eapply MON.
+        -- eapply CMP; eauto. econstructor; eauto.
+            apply H1. 
+         -- intros. apply gpaco2_clo. auto.
+      * pclearbot. apply EqVisUnPrivVisCo; auto.
+        intros. eapply MON.
+        -- eapply CMP; eauto. econstructor; eauto.
+           apply H1. apply H0.
+        -- intros. apply gpaco2_clo. auto.
+      * assert (VisF e1 k0 = observe (Vis e1 k0) ); auto. rewrite H4.
+        remember (Vis e1 k0) as t. constructor; auto; subst. intros.
+        eapply H1; eauto.
+    + constructor; auto. intros. eapply H1; eauto.
+  - remember (VisF e k2) as x.
+    hinduction EQVr before r; intros; subst; try inv Heqx; try inv CHECK; ITrace.inj_existT; subst; 
+    try contradiction; eauto.
+    + pclearbot. remember (TauF t0) as y.
+      hinduction EQVl before r; intros; subst; try inv Heqy; try inv CHECK; ITrace.inj_existT; subst; try contradiction; eauto.
+      * constructor. apply gpaco2_clo. pclearbot. econstructor; eauto.
+        apply H1. admit. (* vclo r problem again *)
+      * eapply EqVisUnPrivTauLCo; eauto. intros. pclearbot.
+        eapply MON.
+        -- eapply CMP; eauto. econstructor; eauto. apply H0.
+           apply H1.
+        -- intros; apply gpaco2_clo; auto.
+      * assert (TauF t1 = observe (Tau t1)); auto. rewrite H4.
+        eapply EqVisUnPrivLInd; eauto. intros. eapply H1; eauto.
+    + pclearbot. remember (TauF t1) as y.
+      hinduction EQVl before r; intros; subst; try inv Heqy; try inv CHECK; ITrace.inj_existT; subst; try contradiction; eauto.
+      * pclearbot. eapply EqVisUnPrivTauRCo; eauto. intros.
+        eapply MON.
+        -- eapply CMP. econstructor; eauto. apply H1.
+        -- intros. apply gpaco2_clo. auto.
+      * constructor; auto. intros. eapply MON.
+        -- eapply CMP. econstructor; eauto. pclearbot.
+           apply H0. apply H1.
+        -- intros. apply gpaco2_clo. auto.
+      * assert (VisF e1 k0 = observe (Vis e1 k0) ); auto.  rewrite H4. eapply EqVisUnPrivLInd; eauto. intros. eapply H1; eauto.
+  - remember (VisF e1 k1) as x.
+    hinduction EQVl before r; intros; inv Heqx; try inv CHECK; ITrace.inj_existT; subst; eauto.
+    + pclearbot. remember (VisF e2 k3) as y. 
+      hinduction EQVr before r; intros; inv Heqy; try inv CHECK; ITrace.inj_existT; subst; eauto.
+      * pclearbot. constructor; eauto. intros.
+        eapply MON.
+        -- eapply CMP. econstructor; eauto. apply H1. apply H0.
+        -- intros. apply gpaco2_clo. auto.
+      * pclearbot. eapply EqVisUnPrivTauLCo; eauto.
+        intros. eapply MON.
+        -- eapply CMP. econstructor; eauto. apply H1. apply H0.
+        -- intros. apply gpaco2_clo. auto.
+      * pclearbot. constructor; eauto. intros.
+        eapply MON.
+        -- eapply CMP. econstructor; eauto. apply H1.
+           apply H0.
+        -- intros. apply gpaco2_clo. auto.
+      * assert (VisF e1 k0 = observe (Vis e1 k0)); auto. rewrite H4.
+       eapply EqVisUnPrivRLInd; eauto. intros. eapply H1; eauto.
+   + pclearbot. remember (VisF e2 k0) as y. 
+     hinduction EQVr before r; intros; inv Heqy; try inv CHECK; ITrace.inj_existT; subst; eauto.
+     * pclearbot.  eapply EqVisUnPrivTauRCo; eauto. intros.
+       eapply MON.
+       -- eapply CMP. econstructor; eauto. apply H1. apply H0.
+       -- intros. apply gpaco2_clo. auto.
+     * constructor. apply gpaco2_clo. econstructor; eauto.
+       apply H1. pclearbot. eapply H0. (* r vclo issue *) admit.
+     * pclearbot. eapply EqVisUnPrivTauRCo; eauto. intros.
+       eapply MON.
+       -- eapply CMP. econstructor; eauto. apply H1. apply H0.
+       -- intros. apply gpaco2_clo. auto.
+     * assert (TauF t3 = observe (Tau t3)); auto. rewrite H4.
+       eapply EqVisUnPrivRLInd; eauto. intros. eapply H1; eauto.
+   + pclearbot. remember (VisF e3 k3) as y.
+     hinduction EQVr before r; intros; inv Heqy; try inv CHECK; ITrace.inj_existT; subst; eauto.
+     * pclearbot. constructor; eauto. intros.
+       eapply MON.
+       -- eapply CMP. econstructor; eauto. apply H1. apply H0.
+       -- intros. apply gpaco2_clo. auto.
+     * pclearbot. eapply EqVisUnPrivTauLCo; eauto. intros.
+       eapply MON.
+       -- eapply CMP. econstructor; eauto. apply H1. apply H0.
+       -- intros. apply gpaco2_clo. auto.
+     * pclearbot. constructor; eauto. intros.
+       eapply MON.
+       -- eapply CMP. econstructor; eauto. apply H1. apply H0.
+       -- intros. apply gpaco2_clo. auto.
+     * assert (VisF e1 k0 = observe (Vis e1 k0)); auto. rewrite H4.
+       eapply EqVisUnPrivRLInd; eauto. intros. eapply H1; eauto.
+ - remember (VisF e k1) as x.
+   hinduction EQVl before r; intros; inv Heqx; try inv CHECK; ITrace.inj_existT; subst; eauto.
+   + pclearbot. constructor; eauto. intros. eapply H2; eauto. specialize (H0 a).
+     punfold H0.
+   + (* using nonempty condition here (note that the weaker (no high sec halts, would also work I think) ) *)
+     assert (nonempty A0); eauto. inv H3.
+     pclearbot. constructor; eauto. eapply H2; eauto. 
+     pstep_reverse.
+   + pclearbot. constructor; eauto. intros.
+     assert (nonempty A0); eauto. inv H3.
+     eapply H2; eauto. specialize H0 with (b := a0). pstep_reverse.  
+ - remember (VisF e k2) as x.
+   hinduction EQVr before r; intros; inv Heqx; try inv CHECK; ITrace.inj_existT; subst; eauto.
+   + pclearbot. constructor; auto. intros.
+     eapply H2; eauto. pstep_reverse.
+   + assert (nonempty A0); auto. inv H3.
+     constructor; auto. eapply H2; eauto. pstep_reverse.
+     pclearbot.
+     eapply H0; auto.
+   + pclearbot. assert (nonempty A0); auto. inv H3.
+     constructor; auto. intros. eapply H2; eauto.
+     specialize H0 with (b := a).
+     pstep_reverse.
+     Unshelve .
+     assert (nonempty A0); auto. 
+Admitted.
+*)
+
+Ltac unpriv_co := try apply EqVisUnPrivVisCo; 
+                  try apply EqVisUnPrivTauLCo; 
+                  try apply EqVisUnPrivTauRCo; 
+                  auto; intros.
+
+Ltac unpriv_ind := try apply EqVisUnPrivLInd;
+                   try apply EqVisUnPrivRInd;
+                   auto; intros.
+
+Ltac gfinal_with H := gfinal; left; apply H.
+
+Ltac ne A := let Hne := fresh "H" in assert (Hne : nonempty A); eauto; inv Hne.
+
+Lemma eqit_secureC_wcompat_id :  forall b1 b2 E R1 R2 (RR : R1 -> R2 -> Prop )
+      Label priv l
+, (forall A (e : E A), (~ leq (priv _ e) l) -> nonempty A) -> wcompatible2 (@secure_eqit_ E R1 R2 Label priv RR b1 b2 l id) 
+                                         (eqit_secureC RR Label priv l b1 b2) .
+Proof.
+  (*Pay attention to where you use the nonempty condition, this might be false*)
+  intros. constructor.
+  { red. intros; eapply eqit_secureC_mon; eauto. }
+  intros. dependent induction PR. 
+  (* figure out the monotone thing*)
+  punfold EQVl. punfold EQVr. red in EQVl. red in EQVr.
+  red in REL. red. hinduction REL before r; intros; clear t1' t2'.
+  - remember (RetF r1) as x. hinduction EQVl before r; intros; subst; try inv Heqx; eauto.
+    remember (RetF r3) as y. hinduction EQVr before r; intros; subst; try inv Heqy; eauto.
+    (* EqVisUnPrivRLInd slight problem with syntactic form of the constructor,
+       nothing deep *)
+    remember (RetF r1) as rr1. assert (rr1 = observe (Ret r1)); subst; auto.
+    rewrite H4. constructor; eauto. intros. eapply H1; eauto.
+  - remember (TauF t1) as x. hinduction EQVl before r; intros; subst; try inv Heqx;
+    try inv CHECK; eauto.
+    + remember (TauF t4) as y. pclearbot. 
+      (* think I might have a lead on the problem, should H0 have vclo not id here?*)
+      hinduction EQVr before r; intros; subst; try inv Heqy;
+      try inv CHECK; pclearbot; eauto.
+      * constructor. gclo. econstructor; eauto with paco.
+      * unpriv_co.
+        gclo. econstructor; eauto with paco. red. auto.
+      * assert (TauF t1 = observe (Tau t1)); auto. rewrite H4. 
+        unpriv_ind. eapply H1; eauto.
+    + pclearbot. remember (TauF t3) as y.
+      hinduction EQVr before r; intros; inv Heqy; try inv CHECK; subst; eauto.
+      -- pclearbot. 
+         unpriv_co. 
+         gclo. econstructor; try apply H0; eauto with paco. apply H1.
+      -- pclearbot. unpriv_co. gclo. 
+         econstructor; try apply H1; try apply H0; eauto with paco.
+      -- rewrite itree_eta' at 1. unpriv_ind. 
+         eapply H1; eauto.
+  - inv CHECK. remember (TauF t1) as x. 
+    hinduction EQVl before r; intros; try inv Heqx; try inv CHECK; subst; eauto. 
+    + constructor; eauto. eapply IHREL; eauto. pclearbot. punfold H0.
+    + constructor; eauto; intros. eapply IHREL; eauto. specialize (H0 a).
+      pclearbot. punfold H0.
+  - inv CHECK. remember (TauF t2) as y.
+    hinduction EQVr before r; intros; try inv Heqy; try inv CHECK; subst; eauto.
+    + constructor; auto. eapply IHREL; eauto. pclearbot. punfold H0.
+    + constructor; auto. intros. specialize (H0 a). pclearbot. punfold H0.
+  - remember (VisF e k1) as x.
+    hinduction EQVl before r; intros; try inv Heqx; try inv CHECK; subst; 
+    ITrace.inj_existT; subst; eauto.
+    + pclearbot. remember (VisF e0 k3) as y.
+      hinduction EQVr before r; intros; try inv Heqy; try inv CHECK; subst;
+      ITrace.inj_existT; subst; eauto.
+      * constructor; auto. intros. red. gclo. pclearbot.
+         econstructor; try apply H0; try apply H1; eauto with paco. gfinal_with H2.
+      * rewrite itree_eta'. pclearbot.
+        unpriv_co.
+        gclo. econstructor; eauto with paco; try apply H1. apply H0. 
+        gfinal_with H2.
+      * pclearbot. unpriv_co.
+        gclo. econstructor; eauto.
+           apply H1. apply H0. gfinal_with H2.
+      * (* inductive case *) rewrite itree_eta' at 1.
+        unpriv_ind. eapply H1; eauto.
+    + pclearbot. remember (VisF e0 k0) as x.
+      hinduction EQVr before r; intros; subst; try inv Heqx; try inv CHECK;
+      ITrace.inj_existT; subst; try contradiction; eauto.
+    + pclearbot. remember (VisF e k3) as x.
+      hinduction EQVr before r; intros; subst; try inv Heqx; try inv CHECK;
+      ITrace.inj_existT; subst; try contradiction; eauto.
+  - remember (VisF e k1) as x. 
+    hinduction EQVl before r; intros; subst; try inv Heqx; try inv CHECK; ITrace.inj_existT; subst; 
+    try contradiction.
+    + constructor; eauto.
+    + pclearbot. remember (TauF t2) as y.
+      hinduction EQVr before r; intros; subst; try inv Heqy; try inv CHECK;
+      ITrace.inj_existT; subst; eauto.
+      * constructor. apply gpaco2_clo. pclearbot.
+        assert (nonempty A0); eauto. inv H3.
+        econstructor; eauto. apply H1. apply H2; auto.
+        Unshelve. auto.
+      * ne A0. unpriv_co. pclearbot.
+         gclo. econstructor; eauto. apply H1.
+         apply H0. gfinal_with H2. Unshelve. auto.
+      * rewrite itree_eta' at 1. unpriv_ind.
+        eapply H1; eauto.
+   + pclearbot. remember (TauF t2) as y.
+      hinduction EQVr before r; intros; subst; try inv Heqy; try inv CHECK;
+      ITrace.inj_existT; subst; eauto.
+      * ne A0.
+        pclearbot. unpriv_co. 
+        intros. gclo. econstructor; eauto.
+        apply H1. gfinal_with H2. 
+      * ne A1.
+        pclearbot. apply EqVisUnPrivVisCo; auto.
+        intros. gclo. econstructor; eauto. apply H1. apply H0.
+        gfinal. left. apply H2. Unshelve. auto. auto.
+      * assert (VisF e1 k0 = observe (Vis e1 k0) ); auto. rewrite H4.
+        remember (Vis e1 k0) as t. constructor; auto; subst. intros.
+        eapply H1; eauto.
+    + constructor; auto. intros. eapply H1; eauto.
+  - remember (VisF e k2) as x.
+    hinduction EQVr before r; intros; subst; try inv Heqx; try inv CHECK; ITrace.inj_existT; subst; 
+    try contradiction; eauto.
+    + pclearbot. remember (TauF t0) as y.
+      hinduction EQVl before r; intros; subst; try inv Heqy; try inv CHECK; ITrace.inj_existT; subst; try contradiction; eauto.
+      * assert (Hne : nonempty A0); eauto. inv Hne.
+        constructor. apply gpaco2_clo. pclearbot. econstructor; eauto.
+        apply H1. apply H2. Unshelve. auto. 
+      * assert (Hne : nonempty A0); eauto. inv Hne.
+        eapply EqVisUnPrivTauLCo; eauto. intros. pclearbot.
+        gclo. econstructor; eauto. apply H0. apply H1. gfinal.
+        left. apply H2. Unshelve. auto.
+      * assert (TauF t1 = observe (Tau t1)); auto. rewrite H4.
+        eapply EqVisUnPrivLInd; eauto. intros. eapply H1; eauto.
+    + pclearbot. remember (TauF t1) as y.
+      hinduction EQVl before r; intros; subst; try inv Heqy; try inv CHECK; ITrace.inj_existT; subst; try contradiction; eauto.
+      * assert (Hne : nonempty A0); eauto. inv Hne.
+        pclearbot. eapply EqVisUnPrivTauRCo; eauto. intros.
+        gclo. econstructor; eauto. apply H1. gfinal. left. apply H2.
+        Unshelve. auto.
+      * assert (Hne : nonempty A1); eauto. inv Hne.
+        constructor; auto. intros. gclo. pclearbot. 
+        econstructor; eauto. apply H0. apply H1. gfinal. left. apply H2.
+        Unshelve. auto.
+      * assert (VisF e1 k0 = observe (Vis e1 k0) ); auto.  rewrite H4. eapply EqVisUnPrivLInd; eauto. intros. eapply H1; eauto.
+  - remember (VisF e1 k1) as x.
+    hinduction EQVl before r; intros; inv Heqx; try inv CHECK; ITrace.inj_existT; subst; eauto.
+    + pclearbot. remember (VisF e2 k3) as y. 
+      hinduction EQVr before r; intros; inv Heqy; try inv CHECK; ITrace.inj_existT; subst; eauto.
+      * assert (Hne : nonempty A0); eauto. inv Hne.
+        assert (Hne : nonempty B); eauto. inv Hne.
+        pclearbot. constructor; eauto. intros.
+        gclo. econstructor; eauto. apply H1. apply H0.
+        gfinal. left. apply H2.
+      * assert (Hne : nonempty B); eauto. inv Hne.
+        pclearbot. eapply EqVisUnPrivTauLCo; eauto.
+        intros. gclo. econstructor; eauto. apply H1. apply H0. gfinal. left. apply H2. 
+        Unshelve. auto.
+      * assert (Hne : nonempty B0); eauto. inv Hne.
+        pclearbot. constructor; eauto. intros. gclo. econstructor; eauto.
+        apply H1. apply H0. gfinal. left. apply H2. Unshelve. auto.
+      * assert (VisF e1 k0 = observe (Vis e1 k0)); auto. rewrite H4.
+        unpriv_ind.
+        eapply H1; eauto.
+   + pclearbot. remember (VisF e2 k0) as y. 
+     hinduction EQVr before r; intros; inv Heqy; try inv CHECK; ITrace.inj_existT; subst; eauto.
+     * assert (Hne : nonempty A0); eauto. inv Hne.
+       pclearbot.  eapply EqVisUnPrivTauRCo; eauto. intros.
+       gclo. econstructor; eauto. apply H1. apply H0. gfinal. left. apply H2.
+       Unshelve. auto.
+     * assert (Hne : nonempty B); eauto. inv Hne.
+       assert (Hne : nonempty A0); eauto. inv Hne.
+       constructor. apply gpaco2_clo. econstructor; eauto.
+       apply H1. pclearbot. eapply H0. apply H2. Unshelve. auto. auto. 
+     * assert (Hne : nonempty B0); eauto. inv Hne.
+       assert (Hne : nonempty A0); eauto. inv Hne.
+       pclearbot. eapply EqVisUnPrivTauRCo; eauto. intros.
+       gclo. econstructor; eauto. apply H1. apply H0.
+       gfinal. left. apply H2. Unshelve. auto. auto.
+     * assert (TauF t3 = observe (Tau t3)); auto. rewrite H4.
+       unpriv_ind. eapply H1; eauto.
+   + pclearbot. remember (VisF e3 k3) as y.
+     hinduction EQVr before r; intros; inv Heqy; try inv CHECK; ITrace.inj_existT; subst; eauto.
+     * assert (Hne : nonempty A1); eauto. inv Hne.
+       pclearbot. constructor; eauto. intros.
+       gclo. econstructor; eauto. apply H1. apply H0. gfinal. left. apply H2.
+       Unshelve. auto.
+     * assert (Hne : nonempty A1); eauto. inv Hne.
+       assert (Hne : nonempty B0); eauto. inv Hne.
+       pclearbot. eapply EqVisUnPrivTauLCo; eauto. intros.
+       gclo. econstructor; eauto. apply H1. apply H0. gfinal. left. apply H2.
+       Unshelve. auto. auto.
+     * assert (Hne : nonempty A1); eauto. inv Hne.
+       assert (Hne : nonempty B0); eauto. inv Hne.
+       pclearbot. constructor; eauto. intros.
+       gclo. econstructor; eauto. apply H1. apply H0. gfinal. left. apply H2.
+       Unshelve. auto. auto.
+     * assert (VisF e1 k0 = observe (Vis e1 k0)); auto. rewrite H4.
+       unpriv_ind. intros. eapply H1; eauto.
+ - remember (VisF e k1) as x.
+   hinduction EQVl before r; intros; inv Heqx; try inv CHECK; ITrace.inj_existT; subst; eauto.
+   + pclearbot. constructor; eauto. intros. eapply H2; eauto. specialize (H0 a).
+     punfold H0.
+   + (* using nonempty condition here (note that the weaker (no high sec halts, would also work I think) ) *)
+     assert (nonempty A0); eauto. inv H3.
+     pclearbot. constructor; eauto. eapply H2; eauto. 
+     pstep_reverse. Unshelve. auto.
+   + pclearbot. constructor; eauto. intros.
+     assert (nonempty A0); eauto. inv H3.
+     eapply H2; eauto. specialize H0 with (b := a0). pstep_reverse.  
+ - remember (VisF e k2) as x.
+   hinduction EQVr before r; intros; inv Heqx; try inv CHECK; ITrace.inj_existT; subst; eauto.
+   + pclearbot. constructor; auto. intros.
+     eapply H2; eauto. pstep_reverse.
+   + assert (nonempty A0); eauto. inv H3.
+     constructor; auto. eapply H2; eauto. pstep_reverse.
+     pclearbot.
+     eapply H0; auto. Unshelve. auto.
+   + pclearbot. assert (nonempty A0); eauto. inv H3.
+     constructor; auto. intros. eapply H2; eauto.
+     specialize H0 with (b := a).
+     pstep_reverse.
+Qed.
+
+Lemma eqit_secure_sym : forall b1 b2 E R1 R2 RR Label priv l (t1 : itree E R1) (t2 : itree E R2),
+    eqit_secure Label priv RR b1 b2 l t1 t2 -> eqit_secure Label priv (flip RR) b2 b1 l t2 t1.
+Proof.
+  intros b1 b2 E R1 R2 RR Label priv l. pcofix CIH.
+  intros t1 t2 Hsec. pfold. red. punfold Hsec. red in Hsec.
+  hinduction Hsec before r; intros; eauto; pclearbot;
+  try (unpriv_co; right; apply CIH; apply H).
+  constructor; auto. intros. right. apply CIH; apply H.
+Qed.
+
+
+(*should try a version of this proof that just plays it straight, once we know it is a PER some extra avenues open up
+  but uggh this proof is going to be a killer
+  *)
+Lemma strong_eqit_secure_trans : forall E (R : Type)
+                  Label priv l (t1 t2 t3: itree E R),
+     (forall (A : Type) (e : E A), ~ leq (priv A e) l -> nonempty A) ->
+    eqit_secure Label priv eq false false l t1 t2 ->
+    eqit_secure Label priv eq false false l t2 t3 ->
+    eqit_secure Label priv eq false false l t1 t3.
+Proof.
+  intros E R Label priv l t1 t2 t3 HE Ht12 Ht23. 
+  eapply gpaco2_init; try eapply eqit_secureC_wcompat_id; eauto with paco.
+  generalize dependent t2. generalize dependent t1. generalize dependent t3.
+  gcofix CIH0. intros. gclo. econstructor; eauto. apply eqit_secure_sym. eauto; intros.
+  - (* back to this question, can I assume something is securely equiv to anything, it is securely equiv to self*) admit.
+  - intros. subst. auto.
+  - intros. red in H. subst. auto.
+Abort.
+
+
+(* maybe I should start by trying to make this above proof smaller *)
+(* I think I need more assumptions from the context*)
+(*not sure how confident I am in this lemma, soon I will try working through it to 
+  see if it works/what goes wrong*)
+Lemma eqit_secure_anything_to_self_aux:
+forall (E : Type -> Type) (R1 : Type) (b1 b2 : bool) (R2 : Type) 
+    (RR : R1 -> R2 -> Prop) (Label : Preorder) (priv : forall x : Type, E x -> L) 
+    (l : L) (A : Type) (r : itree E R1 -> itree E R1 -> Prop),
+  (forall (t1 : itree E R1) (t2 : itree E R2),
+   eqit_secure Label priv RR b1 b2 l t1 t2 -> r t1 t1) ->
+  (forall (t0 : itree E R2) (k1 : A -> itree E R1),
+   (forall a : A, paco2 (secure_eqit_ Label priv RR b1 b2 l id) bot2 (k1 a) t0) ->
+   forall a b : A, r (k1 a) (k1 b)) ->
+  forall (k1 : A -> itree E R1) (a b : A),
+  paco2 (secure_eqit_ Label priv eq b1 b2 l id) r (k1 a) (k1 b).
+Proof.
+  intros E R1 b1 b2 R2 RR Label priv l A r CIH CIH0 k1 a b.
+Abort. 
+(* this would come pretty directly out of a direct transitivity proof *)
+Lemma eqit_secure_anything_to_self : forall b1 b2 E R1 R2 RR Label priv l (t1 : itree E R1) (t2 : itree E R2),
+    (forall (A : Type) (e : E A), ~ leq (priv A e) l -> nonempty A) ->
+    eqit_secure Label priv RR b1 b2 l t1 t2 -> eqit_secure Label priv eq b1 b2 l t1 t1.
+Proof.
+  intros b1 b2 E R1 R2 RR Label priv l t1 t2 Hhalt Ht12. generalize  dependent t2. generalize dependent t1.
+  pcofix CIH. intros. pfold. red. punfold Ht12. red in Ht12. hinduction Ht12 before r; intros; try auto.
+  - pclearbot. constructor. right. eauto.
+  - constructor. left. pfold. apply IHHt12; auto.
+  - pclearbot. constructor; auto. right. eapply CIH; apply H.
+  - pclearbot. apply EqVisUnPrivVisCo; auto.
+    left. revert a b. generalize dependent k1. generalize dependent t0. pcofix CIH0. intros.
+    (* promising addition to coinductive hypothesis?
+
+*)
+    (* if t is no securely equiv to itself, it is securely equiv to nothing? *)
+    admit.
+  (* this case is problematic the coinductive case requires us to consider if the vis chooses diff paths*)
+  - pclearbot. assert (Hne :nonempty A); eauto. inv Hne. constructor. right. eapply CIH.
+    apply H with (a := a).
+  - pclearbot. (* problematic for same reason *) admit.
+  - rewrite itree_eta'. unpriv_ind. pstep_reverse. eapply paco2_mon with (r := bot2); intros; try contradiction. pfold. admit. (* problematic for different but related reason, probably could do a proof similar to the other cases though (assuming those cases are true) just advance coinductively and use H to show that no matter how to continue with k1, you have an equiv tree *)
+  - assert (nonempty A); eauto. inv H1. apply H0; auto.
+Abort.
+ (* although, this might actually not exactly be transitivity when we don't have reflexivity*)
+(* one thing that I think is true and would be helpful, if t is securely equivalent to anything else, it is securely equivalent to itself*)
+
+
+Section Transitivity.
+
+
+  Context (E : Type -> Type) (R : Type) (Label : Preorder) (priv : forall A, E A -> L).
+  Context (l : L).
+  Context (Hhalt_vis : forall A (e : E A), nonempty A -> leq (priv A e) l).
+
+End Transitivity.
 
 End SecureUntimedUnReflexive.
 
@@ -193,4 +801,4 @@ Section SecureTimed.
     match e with TE _ e' a => handle_timed_aux e' a end.
 
 
-End SecureTime.
+End SecureTimed.
