theories/Secure/SecureEqEutt.v
@@ -1,0 +1,196 @@
+From Coq Require Import
+     Arith.PeanoNat
+     Lists.List
+     Strings.String
+     Morphisms
+     Setoid
+     RelationClasses
+     Logic.Classical_Prop
+     Logic.EqdepFacts
+     Program.Equality
+.
+
+From ExtLib Require Import
+     Data.String
+     Structures.Monad
+     Structures.Traversable
+     Data.List.
+
+From ITree Require Import
+     ITree
+     ITreeFacts
+     Events.MapDefault
+     Events.State
+     Events.StateFacts
+     Core.Divergence
+     Dijkstra.TracesIT
+     Secure.SecureEq
+.
+
+From Paco Require Import paco.
+
+Import Monads.
+Import MonadNotation.
+Local Open Scope monad_scope.
+
+Ltac unpriv_co := try apply EqVisUnPrivVisCo; 
+                  try apply EqVisUnPrivTauLCo; 
+                  try apply EqVisUnPrivTauRCo; 
+                  auto; intros.
+
+Ltac unpriv_ind := try apply EqVisUnPrivLInd;
+                   try apply EqVisUnPrivRInd;
+                   auto; intros.
+
+Lemma tau_eqit_secure : forall E R1 R2 Label priv l RR (t1 : itree E R1) (t2 : itree E R2),
+    eqit_secure Label priv RR true true l (Tau t1) t2 -> eqit_secure Label priv RR true true l t1 t2.
+Proof.
+  intros E R1 R2 Label priv l RR.  intros t1 t2 Hsec. pstep. red.
+  punfold Hsec. red in Hsec. cbn in *. remember (TauF t1) as x.
+  hinduction Hsec before priv; intros;  inv Heqx; pclearbot; try inv CHECK; auto.
+  - constructor; auto. pstep_reverse.
+  - unpriv_ind. pstep_reverse.
+Qed.
+
+Lemma unpriv_e_eqit_secure : forall E A R1 R2 Label priv l RR (e : E A) (k : A -> itree E R1) 
+      (t : itree E R2),
+    (~leq (priv A e) l ) ->
+    eqit_secure Label priv RR true true l (Vis e k) t ->
+    forall a, eqit_secure Label priv RR true true l (k a) t.
+Proof.
+  intros. generalize dependent t. rename H into Hunpriv. generalize dependent a.
+  intros. punfold H0. red in H0. cbn in *. pfold. red.
+  remember (VisF e k) as x. genobs_clear t ot.
+  hinduction H0 before l; intros; try inv Heqx; 
+  ITrace.inj_existT; subst; try contradiction;  auto.
+  - constructor; auto. eapply IHsecure_eqitF; eauto.
+  - pclearbot. constructor; auto. pstep_reverse.
+  - unpriv_ind. pstep_reverse. pclearbot. apply H.
+  - unpriv_ind. eapply H0; eauto.
+Qed.
+
+
+(* reformat this lemma? useful but unclear *)
+Lemma eses_aux1: forall (E : Type -> Type) (R2 R1 : Type) (Label : Preorder)
+                    (priv : forall A : Type, E A -> L) (l : L) (RR : R1 -> R2 -> Prop)
+                    (r : itree E R1 -> itree E R2 -> Prop) (m1 m2 : itree E R1),
+              m1 ≈ m2 ->
+               (forall (t1 t1' : itree E R1) (t2 : itree E R2),
+                   t1 ≈ t1' -> eqit_secure Label priv RR true true l t1 t2 -> r t1' t2) ->
+               forall (X : Type) (e : E X) (k : X -> itree E R2),
+                 secure_eqitF Label priv RR true true l id
+                              (upaco2 (secure_eqit_ Label priv RR true true l id) bot2) (observe m1) 
+                              (VisF e k) ->
+                 leq (priv X e) l ->
+                 secure_eqitF Label priv RR true true l id
+                              (upaco2 (secure_eqit_ Label priv RR true true l id) r) (observe m2) 
+                              (VisF e k).
+Proof.
+  intros E R2 R1 Label priv l RR r m1 m2 REL CIH X e k Hsec SECCHECK.
+  remember (VisF e k) as x. punfold REL. red in REL. rewrite Heqx.
+  hinduction Hsec before r; intros; try inv Heqx; ITrace.inj_existT; subst; try contradiction; auto. 
+  - eapply IHHsec; eauto.
+    pstep_reverse. setoid_rewrite <- tau_eutt at 1. pfold. auto.
+  - pclearbot. remember (VisF e0 k1) as y.
+    hinduction REL before r; intros; try inv Heqy; ITrace.inj_existT; subst; auto.
+    + constructor; auto. right. eapply CIH; eauto; try apply H.
+      pclearbot. apply REL.
+    + constructor; eauto.
+  - rewrite H2. remember (VisF e k1) as y.
+    hinduction REL before r; intros; try inv Heqy; ITrace.inj_existT; subst; auto.
+    + pclearbot. rewrite <- H2. unpriv_ind. rewrite H2. eapply H0; eauto.
+      Unshelve. all: auto. pstep_reverse.
+    + constructor; auto. eapply IHREL; eauto.
+Qed.
+
+Lemma eses_aux2:
+forall (E : Type -> Type) (R2 R1 : Type) (Label : Preorder)
+    (priv : forall A : Type, E A -> L) (l : L) (RR : R1 -> R2 -> Prop)
+    (r : itree E R1 -> itree E R2 -> Prop) (m1 m2 : itree E R1) (r0 : R2),
+  m1 ≈ m2 ->
+  secure_eqitF Label priv RR true true l id
+    (upaco2 (secure_eqit_ Label priv RR true true l id) bot2) (observe m1) 
+    (RetF r0) ->
+  secure_eqitF Label priv RR true true l id
+    (upaco2 (secure_eqit_ Label priv RR true true l id) r) (observe m2) 
+    (RetF r0).
+Proof.
+  intros E R2 R1 Label priv l RR r m1 m2 r0 Heutt Hsec.
+  punfold Heutt. red in Heutt. remember (RetF r0) as x.
+  rewrite Heqx. hinduction Hsec before r; intros; inv Heqx; auto.
+  - remember (RetF r1) as y.
+    hinduction Heutt before r; intros; inv Heqy; auto.
+    constructor; auto. eapply IHHeutt; eauto.
+  - eapply IHHsec; eauto. pstep_reverse. rewrite <- tau_eutt at 1. pfold. auto.
+  - remember (VisF e k1) as y. 
+    hinduction Heutt before r; intros; inv Heqy; ITrace.inj_existT; subst; auto.
+    +  unpriv_ind. rewrite H2. eapply H0; eauto. 
+       pclearbot. pstep_reverse.
+    + constructor; auto. eapply IHHeutt; eauto.
+Qed.
+
+Lemma eutt_secure_eqit_secure : forall E Label priv l R1 R2 RR (t1 t1': itree E R1) (t2 : itree E R2),
+    t1 ≈ t1' -> eqit_secure Label priv RR true true l t1 t2 ->
+    eqit_secure Label priv RR true true l t1' t2.
+Proof.
+  intros E Label priv l R1 R2 RR. pcofix CIH. intros t1 t1' t2 Heutt Hsec.
+  punfold Heutt. red in Heutt. punfold Hsec. red in Hsec.
+  pfold. red. hinduction Heutt before r; intros; subst; auto.
+  - remember (RetF r2) as x. hinduction Hsec before r; intros; try inv Heqx; auto.
+    + constructor; auto. eapply IHHsec; eauto.
+    + unpriv_ind. eapply H0; eauto.
+  - genobs_clear t2 ot2. 
+    assert (Ht2 : (exists m3, ot2 = TauF m3) \/ (forall m3, ot2 <> TauF m3) ).
+    { destruct ot2; eauto; right; repeat intro; discriminate. }
+    (* because of the extra inductive cases this is not enough *)
+    destruct Ht2 as [ [m3 Hm3] | Ht2 ].
+    + subst. pclearbot. constructor. right. eapply CIH; eauto.
+      apply tau_eqit_secure. apply eqit_secure_sym. apply tau_eqit_secure.
+      apply eqit_secure_sym. pfold. auto.
+    + destruct ot2; try (exfalso; eapply Ht2; eauto; fail).
+      * pclearbot. rewrite itree_eta' at 1. eapply eses_aux2 with (m1 := Tau m1); eauto. 
+        do 2 rewrite tau_eutt. auto.
+      * assert (leq (priv _ e) l \/ ~ leq (priv _ e) l).
+        { apply classic. }
+        destruct H as [SECCHECK | SECCHECK].
+        ++ pclearbot. rewrite itree_eta' at 1. apply eses_aux1 with (m1 := Tau m1); auto.
+           do 2 rewrite tau_eutt. auto.
+        ++ pclearbot.
+           unpriv_co. pclearbot. right. eapply CIH. apply REL. 
+           apply tau_eqit_secure. 
+           apply eqit_secure_sym.
+           eapply unpriv_e_eqit_secure; eauto.
+           apply eqit_secure_sym. pfold. auto.
+  - pclearbot. rewrite itree_eta' at 1. pstep_reverse.
+    assert (eqit_secure Label priv RR true true l (Vis e k1) t2 ).
+    { pfold; auto. }
+    clear Hsec. rename H into Hsec.
+    destruct (classic (leq (priv _ e) l ) ).
+    + pstep. red. punfold Hsec. red in Hsec.
+      cbn in *. remember (VisF e k1) as x. 
+      hinduction Hsec before r; intros; inv Heqx; ITrace.inj_existT; subst; try contradiction; auto.
+      * constructor; auto. eapply IHHsec; eauto.
+      * constructor; auto; intros. right. eapply CIH; try apply REL. pclearbot. apply H.
+      * rewrite itree_eta' at 1. unpriv_ind. eapply H0; eauto.
+    + punfold Hsec. red in Hsec. pfold. red.
+      cbn in *. (* if its a Tau or a invisible event we are fine*)
+      destruct (observe t2).
+      * inv Hsec. ITrace.inj_existT. subst. unpriv_ind. rewrite H4. rewrite H4 in H1.
+        eapply eses_aux2; eauto. apply REL.
+      * unpriv_co. right. eapply CIH; try apply REL.
+        eapply unpriv_e_eqit_secure; eauto. apply eqit_secure_sym.
+        apply tau_eqit_secure. apply eqit_secure_sym. pfold. auto.
+      * destruct (classic (leq (priv _ e0) l ) ).
+        -- rewrite itree_eta'. unpriv_ind; auto. 
+           inv Hsec; intros; ITrace.inj_existT; subst; try contradiction. cbn.
+           rewrite H5. rewrite H5 in H2. eapply eses_aux1; eauto. apply REL.
+        -- unpriv_co; auto. right. eapply CIH; try apply REL.
+           do 2 (eapply unpriv_e_eqit_secure; eauto; apply eqit_secure_sym).
+           pfold. auto.
+  - eapply IHHeutt; eauto. (* hoist to lemma? *) remember (TauF t0) as x.
+    hinduction Hsec before r;  intros; try inv Heqx; auto.
+    + constructor; auto. pclearbot. pstep_reverse.
+    + constructor; auto. eapply IHHsec; eauto.
+    + pclearbot. unpriv_ind; auto. pstep_reverse.
+    + pclearbot. unpriv_ind. eapply H0; eauto.
+Qed.
